Tests/STLC/__InferSpec.lean
@@ -1,0 +1,80 @@
+import «Lp2lc».Active.STLC.__Infer
+import «Tests».STLC.Fixture
+
+namespace Tests.STLC.Sanity
+
+namespace Trm
+
+open Lp2lc.Active.Util
+open Lp2lc.Active.STLC
+open Tests.STLC.Sanity.Symbolic
+
+section infer
+variable [env : @CompilerEnv Symbolic.I]
+
+example :
+    (vFalse.infer).shouldYields .primitive := by
+  constructor
+  · exact ⟨1, rfl⟩
+  · rfl
+
+example :
+    (primitiveIdFn.infer).shouldYields (.fn .primitive .primitive) := by
+  constructor
+  · exact ⟨2, by simp [AST.Trm.infer, Outcome.map, primitiveIdFn]⟩
+  · rfl
+
+example :
+    (primitiveIdFnOnFalse.infer).shouldYields .primitive := by
+  constructor
+  · refine ⟨3, ?_⟩
+    have hPrimitive : (AST.Typ.primitive : Typ) ≤ .primitive := by
+      rfl
+    simp [AST.Trm.infer, Outcome.map, primitiveIdFnOnFalse, primitiveIdFn, vFalse, hPrimitive]
+  · rfl
+
+example :
+    (get1st.infer).shouldYields (.fn .primitive (.fn .primitive .primitive)) := by
+  constructor
+  · exact ⟨3, by simp [AST.Trm.infer, Outcome.map, get1st]⟩
+  · rfl
+
+example :
+    (get1stOnTuple.infer).shouldYields .primitive := by
+  constructor
+  · refine ⟨5, ?_⟩
+    have hPrimitive : (AST.Typ.primitive : Typ) ≤ .primitive := by
+      rfl
+    simp [AST.Trm.infer, Outcome.map, get1stOnTuple, get1st, vFalse, vTrue, hPrimitive]
+  · rfl
+
+example :
+    (primitiveTrueFnOnFalse.infer).shouldYields .primitive := by
+  constructor
+  · refine ⟨3, ?_⟩
+    have hPrimitive : (AST.Typ.primitive : Typ) ≤ .primitive := by
+      rfl
+    simp [AST.Trm.infer, Outcome.map, primitiveTrueFnOnFalse, primitiveTrueFn, vFalse, hPrimitive]
+  · rfl
+
+example :
+    (Malformed.applyIdFnOnItself.infer).shouldFail := by
+  constructor
+  · refine ⟨3, ?_⟩
+    have hFnNotPrimitive : ¬ ((AST.Typ.fn .primitive .primitive : Typ) ≤ .primitive) := by
+      intro h
+      cases h
+    simp [AST.Trm.infer, Outcome.map, Malformed.applyIdFnOnItself, primitiveIdFn, hFnNotPrimitive]
+  · rfl
+
+example :
+    (Malformed.primitiveApply.infer).shouldFail := by
+  constructor
+  · exact ⟨2, rfl⟩
+  · rfl
+
+end infer
+
+end Trm
+
+end Sanity
