Tests/STLC/package.lean
@@ -3,4 +3,5 @@ import «Tests».STLC.TypDemo
 import «Tests».STLC.TrmDemo
 import «Tests».STLC.Fixture
 import «Tests».STLC.TrmSpec
+import «Tests».STLC.__InferSpec
 import «Tests».STLC.SemanticTypeDemo
